updating

newest/stepWF.v
@@ -11,7 +11,7 @@ Require Import sets.
 Require Import classifiedStep. 
 Require Import Coq.Sets.Powerset_facts. 
 Require Import Heap. 
-(*Require Import ForkIndependence. *)
+Require Import specIndependence. 
 
 Axiom uniqueTP : forall T1 T2 t, tIn (tUnion T1 T2) t -> tIn T1 t -> tIn T2 t -> False. 
 
@@ -83,35 +83,7 @@ Ltac rUnspec := erewrite unspecSingleton; eauto.
 Ltac rUnspecIn H := erewrite unspecSingleton in H; eauto.
 Ltac rUnspecAll := erewrite unspecSingleton in *; eauto. 
 
-Inductive eraseTrm : list action -> trm -> trm -> Prop :=
-|eraseTrmNil : forall M, eraseTrm nil M M
-|eraseTrmRead : forall x t E d s M, eraseTrm (s++[rAct x t E d]) M t
-|eraseTrmWrite : forall x t E M d N s, eraseTrm (s++[wAct x t E M d]) N t
-|eraseTrmNew : forall x t E d s M, eraseTrm (s++[nAct t E d x]) M t
-|eraseTrmFork : forall t E M d N s, eraseTrm (s++[fAct t E M d]) N t
-|eraseTrmSR : forall t E M N d M' s, eraseTrm (s++[srAct t E M N d]) M' t. 
 
-Theorem unspecEraseTrm : forall tid s1 s2 M M', 
-                          eraseTrm s1 M M' ->
-                          unspecThread(tid,unlocked s1,s2,M) (tSingleton(tid,unlocked nil,s2,M')). 
-Proof.
-  intros. destructLast s1. 
-   {inv H; try invertListNeq. auto. }
-   {invertHyp. inv H; try solve[invertListNeq]; apply lastElementEq in H1;
-   subst; unspecThreadTac; auto. }
-Qed. 
-
-Theorem eEraseTrm : forall s1 M, exists M', eraseTrm s1 M M'. 
-  intros. destructLast s1. 
-  {econstructor. econstructor. }
-  {invertHyp. destruct x; econstructor; econstructor. }
-Qed. 
-
-Ltac eraseTrmTac s1 M := assert(exists M', eraseTrm s1 M M') by apply eEraseTrm; invertHyp.  
-
-Theorem EqJMeq : forall (T:Type) (x y:T), x = y -> JMeq x y.
-Proof.
-  intros. subst. auto. Qed. 
 
 Axiom UnionSingletonEq : forall T T' a b, 
                  tUnion T (tSingleton a) = tUnion T' (tSingleton b) -> 
@@ -131,237 +103,144 @@ Axiom UnionSingletonCoupleEq : forall T T' a b c,
 
 Axiom CoupleUnionAx : forall T T' t1 t2,
                         tUnion T (tSingleton t1) = tUnion T' (tCouple t1 t2) -> 
-                        T = tUnion T' (tSingleton t2). 
+                        T = tUnion T' (tSingleton t2).
 
-
-Theorem simSpecJoin : forall H T H' T' tid s1 s2 M' M'',
-                        spec_multistep H (tUnion T (tSingleton(tid,s1,s2,M'))) H' 
-                                       (tUnion T' (tSingleton(tid,s1,s2,M''))) ->
-                        spec_multistep H T H' T'. 
-Proof.
-  intros. dependent induction H0. 
-  {unfoldTac. apply UnionEqTID in x. invertHyp. constructor. }
-  {copy x. unfoldSetEq x. copy H. apply specStepSingleton in H4. invertHyp. 
-   assert(tIn (tUnion T0 (tSingleton x)) x). apply Union_intror. constructor.
-   apply H2 in H4. inv H4. 
-   {copy H5. apply pullOut in H5. rewrite H5. econstructor. eapply specStepChangeUnused. 
-    eauto. eapply IHspec_multistep. Focus 2. auto. apply UnionSingletonEq in H1. rewrite H1. 
-    unfoldTac. rewrite UnionSwap. auto. auto. }
-   {inv H5. inv H. 
-    {unfoldTac; invertHyp. inv H4. eapply IHspec_multistep; eauto. apply UnionEqTID in H1. 
-     invertHyp. auto. }
-     {unfoldTac; invertHyp. inv H7. eapply monotonicActions in H0. Focus 2. 
-      apply Union_intror. constructor. Focus 2. apply Union_intror. constructor.
-      destruct s1; simpl in *; omega. }
-     {unfoldTac; invertHyp. inv H4. eapply monotonicActions in H0. Focus 2. 
-      apply Union_intror. constructor. Focus 2. apply Union_intror. constructor.
-      destruct s1; simpl in *; omega. }
-     {unfoldTac; invertHyp. inv H4. eapply monotonicActions in H0. Focus 2. 
-      apply Union_intror. constructor. Focus 2. apply Union_intror. constructor.
-      destruct s1; simpl in *; omega. }
-     {unfoldTac; invertHyp. inv H4. eapply monotonicActions in H0. Focus 2. 
-      apply Union_intror. constructor. Focus 2. apply Union_intror. constructor.
-      destruct s1; simpl in *; omega. }
-     {unfoldTac; invertHyp. inv H7. eapply monotonicActions in H0. Focus 2. 
-      apply Union_intror. constructor. Focus 2. apply Union_intror. constructor.
-      destruct s1; simpl in *; omega. }
-    }
-  }
-Qed. 
-
-Theorem wrapDistributeApp : forall s a N E e p, 
-                              wrapActs(s++[a]) N E e p = wrapActs(s) N E e p++ wrapActs[a] N E e p.
-Proof.
-  induction s; intros. 
-  {simpl. destruct a; auto. }
-  {simpl. destruct a; auto; destruct a0; auto; rewrite IHs; auto. }
-Qed. 
-
-Theorem wrapEraseTrm : forall s M M' N N' E p,
-                         eraseTrm s M M' -> 
-                         eraseTrm (wrapActs s N E N' p) 
-                                  (fill E (specJoin (ret N) M)) (fill E (specJoin (ret N) M')). 
-Proof.
-  intros. inv H; try solve[rewrite wrapDistributeApp; constructor]. 
-  {simpl. constructor. }
-Qed. 
-
-
-Ltac specActEq H := 
-  eapply firstSpecActEq in H; [idtac|apply Union_intror; rewrite app_nil_l; constructor|
-                               apply Union_intror; constructor]. 
-
-Theorem eraseTrmApp : forall x a M M', 
-                        eraseTrm (x ++ [a]) M M' -> actionTerm a M'. 
-Proof.
-  intros. inv H; try solve[apply lastElementEq in H1; subst; constructor].
-  invertListNeq. 
-Qed. 
-
-Theorem specFastForward : forall H T H' T' tid x0 x s2' N N0 M M' M'',
-             eraseTrm (x0++[x]) N M' ->                                                
-             spec_multistep H (tUnion T (tSingleton(tid,specStack nil N0, s2', M)))
-                            H' (tUnion T' (tSingleton(tid,specStack(x0++[x]) N0, s2', M''))) ->
-             exists H'' T'',
-               spec_multistep H (tUnion T (tSingleton(tid,specStack nil N0, s2', M))) 
-                              H'' (tUnion T'' (tSingleton(tid,specStack nil N0, s2', M'))) /\
-               spec_multistep H'' (tUnion T'' (tSingleton(tid, specStack nil N0, s2', M')))
-                              H' (tUnion T' (tSingleton(tid,specStack(x0++[x]) N0, s2',M''))). 
+Ltac actEqTac H :=
+  eapply firstActEq in H;[idtac|apply Union_intror; rewrite app_nil_l; constructor|
+                          apply Union_intror; constructor]. 
+Theorem forkFastForward : forall H T H' T' tid s1' s1'' N M M' M'' E s2 d,
+  decompose M' E (fork M'') ->                                            
+  spec_multistep H (tUnion T (tSingleton(tid,unlocked nil, s2, M')))
+                 H' (tUnion T' (tCouple(tid,unlocked(s1'++[fAct M' E M'' d]),s2,M)
+                                       (1::tid,locked s1'',nil,N))) ->
+  exists H'' T'',
+    spec_multistep H (tUnion T (tSingleton(tid,unlocked nil,s2,M')))
+                   H'' (tUnion T'' (tCouple(tid,unlocked[fAct M' E M'' d],s2,fill E (ret unit))
+                                          (1::tid,locked nil,nil,M''))) /\
+    spec_multistep H'' (tUnion T'' (tCouple(tid,unlocked[fAct M' E M'' d],s2,fill E (ret unit)) (1::tid,locked nil,nil,M'')))
+                   H'(tUnion T' (tCouple(tid,unlocked(s1'++[fAct M' E M'' d]),s2,M)
+                                       (1::tid,locked s1'',nil,N))) /\
+    spec_multistep H T H'' T''. 
 Proof.
   intros. dependent induction H1. 
-  {apply UnionEqTID in x. invertHyp. inv H. invertListNeq. }
-  {copy x. unfoldSetEq H2. copy H. apply specStepSingleton in H2. invertHyp. 
-   assert(tIn (tUnion T0 (tSingleton x2)) x2). apply Union_intror. constructor. apply H3 in H2. 
-   inv H2. 
-   {eapply IHspec_multistep in H0. Focus 3. auto. Focus 2. apply UnionSingletonEq in x; auto.  
-    rewrite x. unfoldTac. rewrite UnionSwap. auto. invertHyp. exists x3. exists x4. split; auto.
-    apply pullOut in H5. unfoldTac. rewrite H5. rewrite UnionSwap. econstructor. 
-    eapply specStepChangeUnused. eauto. unfoldTac. rewrite <- UnionSwap. eauto. }
-   {inv H5. apply UnionEqTID in x. invertHyp. clear H2 H5 H7. inversion H; subst. 
-    {unfoldTac; invertHyp. inv H2. eapply IHspec_multistep in H0. Focus 3. 
-     auto. Focus 2. auto. invertHyp. exists x. exists x2. split; eauto. econstructor. 
-     eapply SBasicStep; eauto. assumption. }
-    {unfoldTac; invertHyp. inv H7. copy H1. specActEq H1. subst. 
-     apply eraseTrmApp in H0. inv H0.  exists h'. exists T. split. constructor. 
-     econstructor. eapply SFork. eauto. }
-    {unfoldTac; invertHyp. inv H2. copy H1. specActEq H1. subst. exists h. exists T. 
-     apply eraseTrmApp in H0. inv H0. split. constructor. econstructor. 
-     eauto. eauto. }
-    {unfoldTac; invertHyp. inv H2. copy H1. specActEq H1. subst. exists h. exists T. 
-     apply eraseTrmApp in H0. inv H0. split. constructor. econstructor. 
-     eauto. eauto. }
-    {unfoldTac; invertHyp. inv H2. copy H1. specActEq H1. subst. exists h. exists T. 
-     apply eraseTrmApp in H0. inv H0. split. constructor. econstructor. 
-     eauto. eauto. }
-    {unfoldTac; invertHyp. inv H7. copy H1. specActEq H1. subst. apply eraseTrmApp in H0. 
-     inv H0. exists h'. exists T. split. constructor. econstructor. eauto. eauto. }
-   }
-  }
-Qed. 
-
-Ltac monoActs H :=
-  eapply monotonicActions in H;[idtac|apply Union_intror; constructor|apply Union_intror;constructor].
-
-Theorem simTSteps : forall H T H' T' tid s1 s2 s1' s2' N M M' tid',
-                      spec_multistep H (tUnion T (tSingleton(tid,s1,s2,M)))
-                                     H' (tUnion T' (tSingleton(tid,s1,s2,M'))) ->
-                      spec_multistep H (tUnion T (tSingleton(tid',s1',s2',N)))
-                                     H' (tUnion T' (tSingleton(tid',s1',s2',N))). 
-Proof.
-  intros. dependent induction H0. 
-  {apply UnionEqTID in x. invertHyp. constructor. }
-  {copy x. unfoldSetEq x. copy H. apply specStepSingleton in H4. invertHyp. 
-   assert(tIn (tUnion T0 (tSingleton x)) x). apply Union_intror. constructor. 
-   apply H2 in H4. inv H4. 
-   {copy H5. apply pullOut in H5. rewrite H5. unfoldTac. rewrite UnionSwap. econstructor. 
-    eapply specStepChangeUnused. eauto. unfoldTac. rewrite <- UnionSwap.
-    eapply IHspec_multistep; eauto. apply UnionSingletonEq in H1. rewrite H1.
-    rewrite UnionSwap. eauto. auto. }
-   {inv H5. inv H; unfoldTac; invertHyp; invThreadEq.   
-    {eapply IHspec_multistep; eauto. apply UnionEqTID in H1. invertHyp. eauto. }
-    {monoActs H0. destruct s1; simpl in *; omega. }
-    {monoActs H0. destruct s1; simpl in *; omega. }
-    {monoActs H0. destruct s1; simpl in *; omega. }
-    {monoActs H0. destruct s1; simpl in *; omega. }
-    {monoActs H0. destruct s1; simpl in *; omega. }
-   }
-  }
-Qed. 
-
-Fixpoint joinCtxts E1 E2 :=
-  match E1 with
-      | bindCtxt E M => bindCtxt (joinCtxts E E2) M
-      | handleCtxt E M => handleCtxt (joinCtxts E E2) M
-      | appCtxt E M => appCtxt (joinCtxts E E2) M
-      | appValCtxt E M => appValCtxt (joinCtxts E E2) M
-      | pairCtxt E M => pairCtxt (joinCtxts E E2) M
-      | pairValCtxt E M => pairValCtxt (joinCtxts E E2) M
-      | fstCtxt E => fstCtxt (joinCtxts E E2)
-      | sndCtxt E => sndCtxt (joinCtxts E E2)
-      | specRunCtxt E M => specRunCtxt (joinCtxts E E2) M
-      | specJoinCtxt E M => specJoinCtxt (joinCtxts E E2) M
-      | holeCtxt => E2
-  end. 
-
-Theorem notValFill : forall E e, ~ val e -> ~val (fill E e). 
-Proof.
-  induction E; intros; simpl; try solve[introsInv].
-  {intros c. inv c. apply IHE in H. contradiction. }
-  {intros c. inv c. apply IHE in H. contradiction. }
-  {auto. }
-Qed. 
-
-Theorem decomposeNotVal : forall t E e, decompose t E e -> E <> holeCtxt -> ~val t. 
-Proof.
-  intros. induction H; try solve[introsInv].
-  {intros c. inv c. contradiction. }
-  {introsInv. contradiction. }
-Qed. 
-
-Theorem decomposeFurther : forall E E' e e' e'',
-                                  ctxtWF e E -> decompose e' E' e'' -> ~ val e' ->
-                                  decompose (fill E e') (joinCtxts E E') e''.
-Proof.
-  induction E; intros. 
-  {simpl. constructor. inv H. eapply notValFill. auto. inv H. eapply IHE; eauto. }
-  {simpl. inv H. constructor. auto. apply notValFill; auto. eauto. }
-  {inv H. simpl. constructor; eauto. apply notValFill; eauto. }
-  {inv H. simpl. constructor; eauto. apply notValFill; eauto. }
-  {inv H. simpl. constructor; eauto. apply notValFill; eauto. }
-  {inv H. simpl. constructor; eauto. apply notValFill; eauto. }
-  {inv H. simpl. constructor; eauto. apply notValFill; eauto. }
-  {inv H. simpl. constructor; eauto. apply notValFill; eauto. }
-  {inv H. simpl. constructor; eauto. apply notValFill; eauto. }
-  {inv H. simpl. constructor; eauto. apply notValFill; eauto. }
-  {simpl. auto. }
-Qed. 
-
-
-Theorem joinFill : forall E1 E2 e, fill (joinCtxts E1 E2) e = fill E1 (fill E2 e). 
-Proof.
-  induction E1; intros; try solve[simpl; rewrite IHE1; eauto]. 
-  simpl. auto. 
-Qed. 
-
-Theorem simBasicStepFill : forall E e M M',
-                             ctxtWF e E -> basic_step M M' ->
-                             basic_step (fill E M) (fill E M'). 
-Admitted. 
-
-Theorem simSpecJoin' : forall H T H' T' tid tid' s2 s2' M M' s1 s1' N0 N1 E e p,              
-        spec_multistep H (tUnion T (tSingleton(tid,specStack s1 N0, s2, M)))
-                       H' (tUnion T' (tSingleton(tid,specStack s1' N0, s2, M'))) -> ~val e ->
-        spec_multistep H (tUnion T (tSingleton(tid',unlocked (wrapActs s1 N1 E e p),s2',fill E (specJoin(ret N1)M))))
-           H' (tUnion T' (tSingleton(tid',unlocked(wrapActs s1' N1 E e p),s2',fill E (specJoin(ret N1)M')))).
-Proof.
-  intros. dependent induction H0. 
-  {apply UnionEqTID in x. invertHyp. inv H. constructor. }
+  {unfoldTac. rewrite coupleUnion in x. rewrite <- Union_associative in x. 
+   rewrite UnionSwap in x. apply UnionEqTID in x. invertHyp. inv H. invertListNeq. }
   {copy x. unfoldSetEq H2. copy H. apply specStepSingleton in H2. invertHyp. 
    assert(tIn (tUnion T0 (tSingleton x0)) x0). apply Union_intror. constructor. 
    apply H3 in H2. inv H2. 
-   {copy H5. apply pullOut in H5. rewrite H5. unfoldTac. rewrite UnionSwap. econstructor. 
-    eapply specStepChangeUnused. eauto. unfoldTac. rewrite <- UnionSwap.
-    eapply IHspec_multistep; eauto. apply UnionSingletonEq in x; auto.  rewrite x. 
-    rewrite UnionSwap. auto. }
-   {inv H5. apply UnionEqTID in x. invertHyp. inv H; unfoldTac; invertHyp; invThreadEq.  
-    {inv H8. 
-     {econstructor. eapply SBasicStep; auto. eapply basicBeta.  
+   {eapply IHspec_multistep in H0. Focus 3. auto. Focus 2. 
+    apply UnionSingletonEq in x; auto.  
+    rewrite x. unfoldTac. rewrite UnionSwap. auto. invertHyp. exists x1. exists x2.
+    split; auto. apply pullOut in H5. unfoldTac. rewrite H5. rewrite UnionSwap. 
+    econstructor. eapply specStepChangeUnused. eauto. unfoldTac. 
+    rewrite <- UnionSwap. eauto. split. auto. copy H5. apply pullOut in H5. 
+    rewrite H5. econstructor. eapply specStepChangeUnused. eauto. eauto. }
+   {inv H5. apply UnionEqTID in x. invertHyp. clear H2 H5 H7. inversion H; subst. 
+    {unfoldTac; invertHyp; invThreadEq.
+     inv H5; eapply uniqueCtxtDecomp in H0; eauto; invertHyp; solveByInv. }
+    {unfoldTac; invertHyp; invThreadEq. copy d0. eapply uniqueCtxtDecomp in H0; eauto.
+     invertHyp. inv H6. exists h'. exists T. split. econstructor. 
+     eapply SFork; eauto. constructor. copy H1. simpl in *. assert(d=d0). 
+     apply proof_irrelevance. subst. split. eassumption. constructor. }
+    {unfoldTac; invertHyp; invThreadEq. copy d0; eapply uniqueCtxtDecomp in H0; eauto.
+     invertHyp. inv H7. }
+    {unfoldTac; invertHyp; invThreadEq. copy d0; eapply uniqueCtxtDecomp in H0; eauto.
+     invertHyp. inv H7. }
+    {unfoldTac; invertHyp; invThreadEq. copy d0; eapply uniqueCtxtDecomp in H0; eauto.
+     invertHyp. inv H6. }
+    {unfoldTac; invertHyp; invThreadEq. copy d0; eapply uniqueCtxtDecomp in H0; eauto.
+     invertHyp. inv H6. }
+   }
+  }
+Qed. 
 
-Theorem decomposeFill : forall e e' e'' E E', 
-                          ctxtWF e E -> decompose e' E' e'' -> ~val e'' ->
-                          decompose (fill E e') (joinCtxts E E') e''. 
+Theorem appCons : forall (T:Type) x (y:T) z,
+                    x ++ [y;z] = (x ++ [y]) ++ [z]. 
+Proof. 
+  intros. rewrite <- app_assoc. simpl. auto. Qed. 
+
+Theorem consedActEq : forall H H' tid s1 s1' a b s2 M M' T T',
+                 spec_multistep H T H' T' -> tIn T (tid,unlocked (s1++[a;b]),s2,M) -> 
+                 tIn T' (tid,unlocked(s1'++[b]),s2,M') -> exists s, s1' = s ++ [a]. 
 Proof.
-  intros. induction H. 
-  {simpl. 
+(*
+  intros. genDeps{s1';s1;s2;a;b;c;M;M';tid}. induction H0; intros. 
+  {assert(thread_lookup p2 tid (tid,unlocked(s1++[a;b]),s2,M)). econstructor. eauto. auto. 
+   assert(thread_lookup p2 tid (tid,unlocked(s1'++[c;b]),s2,M')). econstructor. eauto. auto.
+   eapply uniqueThreadPool in H; eauto. inv H. replace [a;b] with ([a]++[b]) in H4; auto. 
+   replace [c;b] with ([c]++[b]) in H4; auto. repeat rewrite app_assoc in H4. 
+   apply app_inj_tail in H4. inv H4. apply lastElementEq in H. subst. auto. }
+  {inv H1. 
+   {eapply IHspec_multistep. constructor. eauto. eauto. }
+   {copy H. apply specStepSingleton in H. invertHyp. inv H3. inv H1. 
+    {unfoldTac; invertHyp. inv H. eapply IHspec_multistep. apply Union_intror. constructor. eauto. }
+    {unfoldTac; invertHyp. inv H5. eapply IHspec_multistep. apply Union_intror. simpl. 
+     rewrite app_comm_cons. constructor. eauto. }
+    {unfoldTac; invertHyp. inv H. eapply IHspec_multistep. apply Union_intror. simpl. 
+     rewrite app_comm_cons. constructor. eauto. }
+    {unfoldTac; invertHyp. inv H. eapply IHspec_multistep. apply Union_intror. simpl. 
+     rewrite app_comm_cons. constructor. eauto. }
+    {unfoldTac; invertHyp. inv H. eapply IHspec_multistep. apply Union_intror. simpl. 
+     rewrite app_comm_cons. constructor. eauto. }
+    {unfoldTac; invertHyp. inv H5. eapply IHspec_multistep. apply Union_intror. simpl. 
+     rewrite app_comm_cons. constructor. eauto. }
+   }
+  }
+Qed.*) 
+Admitted. 
 
+Theorem eraseTrmActTerm : forall x a M M',
+                            eraseTrm (x++[a]) M M' ->
+                            actionTerm a M'. 
+Proof.
+  intros. destruct a; inv H; try solve[invertListNeq]; 
+  apply lastElementEq in H1; inv H1; constructor. 
+Qed. 
 
-
-
-
-
-
-
-
+Theorem forkCatchup : forall H T H' T' x x0 tid s1' s1'' s2 e1 e1' e2 e2' M' M'' E d,
+    eraseTrm s1' e1' x -> eraseTrm s1'' e2' x0 ->
+    spec_multistep H (tUnion T (tCouple(tid,unlocked[fAct M' E M'' d], s2, e1)
+                                       (1::tid,locked nil,nil,e2)))
+                   H' (tUnion T' (tCouple(tid,unlocked(s1'++[fAct M' E M'' d]),s2,e1')
+                                         (1::tid,locked s1'',nil,e2'))) -> 
+    exists H'' T'',
+      spec_multistep H (tUnion T (tCouple(tid,unlocked[fAct M' E M'' d],s2,e1)
+                                         (1::tid,locked nil,nil,e2)))
+                     H'' (tUnion T'' (tCouple(tid,unlocked[fAct M' E M'' d],s2,x)
+                                             (1::tid,locked nil,nil,x0))) /\
+      spec_multistep H'' (tUnion T'' (tCouple(tid,unlocked[fAct M' E M'' d],s2,x)
+                                             (1::tid,locked nil,nil,x0)))
+                 H' (tUnion T' (tCouple(tid,unlocked(s1'++[fAct M' E M'' d]),s2,e1')
+                                         (1::tid,locked s1'',nil,e2'))) /\
+      spec_multistep H T H'' T''. 
+Proof.
+  intros. genDeps{x;x0}. dependent induction H2; intros.
+  {unfoldTac. repeat rewrite coupleUnion in x. 
+   repeat rewrite <- Union_associative in x. apply UnionEqTID in x. invertHyp. 
+   inv H3. apply UnionEqTID in H. invertHyp. inv H. destruct s1'; inv H5. 
+   inv H0; try invertListNeq. inv H1; try invertListNeq. exists h. exists T'. 
+   split. constructor. split. constructor. constructor. invertListNeq. }
+  {copy x. copy H. apply specStepSingleton in H4. invertHyp. copy x. unfoldSetEq x.
+   assert(tIn (tUnion T0 (tSingleton x2)) x2). apply Union_intror. constructor.
+   apply H5 in H7. inv H7. 
+   {eapply IHspec_multistep in H0; eauto. invertHyp. exists x. exists x3. 
+    split. copy H8. apply pullOut in H9. rewrite H9. unfoldTac. rewrite UnionSwap. 
+    econstructor. eapply specStepChangeUnused. eauto. unfoldTac. rewrite <- UnionSwap.
+    eauto. split. auto. copy H8. apply pullOut in H9. rewrite H9. econstructor. 
+    eapply specStepChangeUnused. eauto. auto. apply UnionSingletonCoupleEq in H3. 
+    rewrite H3. unfoldTac. rewrite UnionSwap. auto. auto. }
+   {inv H8. unfoldTac. rewrite coupleUnion in H3. rewrite <- Union_associative in H3.
+    rewrite UnionSwap in H3. apply UnionEqTID in H3. invertHyp. 
+    inv H; unfoldTac; invertHyp; invThreadEq. 
+    {eapply IHspec_multistep in H0. invertHyp. exists x. exists x2. 
+     split. rewrite coupleUnion. rewrite <- Union_associative. rewrite UnionSwap. 
+     econstructor. eapply SBasicStep. eauto. constructor. unfoldTac. 
+     rewrite <- UnionSwap. rewrite Union_associative. rewrite <- coupleUnion. 
+     eauto. split. eassumption. assumption.  rewrite Union_associative. 
+     rewrite <- coupleUnion. rewrite couple_swap. auto. auto. auto. }
+    {simpl in *. eapply consedActEq in H2. Focus 2. apply Union_intror. simpl. 
+     rewrite app_nil_l. constructor. Focus 2. apply Union_intror. constructor. 
+     invertHyp. copy H0. apply eraseTrmActTerm in H0. inv H0. 
 
 
 Theorem stepWF : forall H T t H' t', 
@@ -482,7 +361,7 @@ Proof.
    {unfoldTac. rewrite coupleUnion in *. repeat rewrite unspecUnionComm in *. simpl. 
     repeat rUnspecAll. unfoldTac. repeat rewrite union_empty_r in *. eapply spec_multi_trans. 
     eassumption. econstructor. eapply SSpec; eauto. rewrite <- coupleUnion. constructor. }
-  }
+  }  
   {inv H0. inv H2. econstructor; eauto. unfoldTac. rewrite couple_swap in H3. 
    rewrite coupleUnion in H3. repeat rewrite unspecUnionComm in *. 
    erewrite unspecSingleton in H3; eauto. erewrite unspecSingleton in H3; eauto. 
@@ -494,7 +373,8 @@ Proof.
     eapply wrapEraseTrm with(N:=N1)(E:=E)(N':=(specRun(ret N1) N0))in H0.
     erewrite unspecSingleton. Focus 2. apply unspecEraseTrm; eauto.
     eapply specFastForward in H3; eauto. invertHyp. eapply spec_multi_trans. 
-    eapply simTSteps in H2. eassumption. eapply simSpecJoin' in H4. simpl in *. eauto. }
+    eapply simTSteps in H2. eassumption. eapply simSpecJoin' in H4. simpl in *.
+    eauto. eauto. constructor. introsInv. }
   }
   {copy H13. unfoldTac. rewrite <- Union_associative. rewrite wfFrame. Focus 2. 
    unfold commitPool. intros. inv H3. auto. rewrite <- Union_associative in H0. 
@@ -502,23 +382,29 @@ Proof.
    eapply rollbackWF; eauto. }
   {inv H0. inv H2. econstructor; eauto. rewrite unspecUnionComm in *. rUnspecAll. 
    rewrite spec_multi_unused in H3. rewrite spec_multi_unused. auto. }
-  {inversion H0; subst. inversion H3; subst. econstructor; eauto. erewrite unspecHeapRBRead; eauto. 
-   rewrite unspecUnionComm in *. erewrite unspecSingleton in H4. Focus 2. 
-   unspecThreadTac; auto. eraseTrmTac s1' M. erewrite unspecSingleton. Focus 2. 
-   eapply unspecEraseTrm; eauto. eapply specStepRead in H4; eauto. Focus 2. 
-   eapply lookupUnspecFull; eauto. invertHyp. rewrite unspecUnspecHeap in H2. 
-   rewrite unspecUnspecPool in H7. rewrite <- H2. inv H7. 
+  {inv H0. inv H3. econstructor; eauto. erewrite unspecHeapRBRead; eauto. 
+   admit. }
+  {inv H0. inv H3. econstructor; eauto. unfoldTac. admit. }
+  {admit. }
+  {admit. }
+  {inv H0. inv H2. econstructor; eauto. unfoldTac. rewrite coupleUnion in *. 
+   repeat rewrite unspecUnionComm in *. eraseTrmTac s1' M. rUnspecAll. 
+   Focus 2. unspecThreadTac; eauto. Focus 3. unspecThreadTac; eauto. 
+   Focus 2. apply unspecEraseTrm; eauto. eraseTrmTac s1'' N. rUnspecAll. Focus 2. 
+   apply unspecEraseTrm. eauto. unfoldTac. rewrite union_empty_r in H3. 
+   rewrite <- coupleUnion in H3. eapply forkFastForward in H3; eauto. invertHyp.
+   eapply spec_multi_trans. erewrite spec_multi_unused. eassumption. 
+   repeat rewrite <- coupleUnion. eapply forkCatchup in H3; eauto. 
+   invertHyp. eapply spec_multi_trans. rewrite spec_multi_unused. eassumption. 
    
-  {inv H0. inv H2. econstructor; eauto. unfoldTac. rewrite coupleUnion in *.
-   repeat rewrite unspecUnionComm in *. erewrite unspecSingleton in H3. Focus 2. 
-   eapply unspecFork; auto. erewrite unspecSingleton in H3. Focus 2. 
-   eapply unspecLocked; eauto. unfoldTac. rewrite union_empty_r in H3. 
-   rewrite <- coupleUnion in H3. apply forkInd' in H3. unfoldTac. rewrite coupleUnion in H3. 
-   rewrite unspecUnionComm in H3. eauto. }
-
-                    
-
-a;lkhdj
+   
 
 
 
+
+  
+
+
+
+
+aldsfhlasdkjhfasd
