newest/specIndependence.v
@@ -1,0 +1,416 @@
+Require Import SfLib.           
+Require Import NonSpec.   
+Require Import Spec.  
+Require Import Coq.Sets.Ensembles. 
+Require Import erasure. 
+Require Import AST. 
+Require Import hetList. 
+Require Import Coq.Program.Equality. 
+Require Import unspec. 
+Require Import sets. 
+Require Import classifiedStep. 
+Require Import Coq.Sets.Powerset_facts. 
+Require Import Heap. 
+
+Axiom uniqueTP : forall T1 T2 t, tIn (tUnion T1 T2) t -> tIn T1 t -> tIn T2 t -> False. 
+
+Theorem unionEq : forall T1 T2 T2', tUnion T1 T2 = tUnion T1 T2' -> T2 = T2'.  
+Proof.
+  intros. apply Extensionality_Ensembles. unfold Same_set. unfold Included. split; intros. 
+  {apply eqImpliesSameSet in H. unfold Same_set in H. unfold Included in H. inv H. 
+   assert(tIn (tUnion T1 T2) x). apply Union_intror. auto. copy H. apply H1 in H.
+   inversion H; subst. eapply uniqueTP in H0; eauto. inversion H0. auto. }
+  {apply eqImpliesSameSet in H. unfold Same_set in H. unfold Included in H. inv H. 
+   assert(tIn (tUnion T1 T2') x). apply Union_intror. auto. copy H. apply H2 in H3. 
+   inversion H3; subst. eapply uniqueTP in H0; eauto. inversion H0. auto. }
+Qed. 
+
+Theorem UnionEqTID : forall T T' tid s1 s2 M s1' s2' M',
+                       tUnion T (tSingleton(tid,s1,s2,M)) = tUnion T' (tSingleton(tid,s1',s2',M')) ->
+                       T = T' /\ s1 = s1' /\ s2 = s2' /\ M = M'. 
+Proof. 
+  intros. unfoldSetEq H. assert(tIn (tUnion T (tSingleton(tid,s1,s2,M)))(tid,s1,s2,M)). 
+  apply Union_intror. constructor. copy H.  apply H0 in H. inversion H.  
+  {assert(thread_lookup (tUnion T' (tSingleton(tid,s1',s2',M'))) tid (tid,s1,s2,M)). 
+   econstructor. econstructor. eauto. auto. 
+   assert(thread_lookup (tUnion T' (tSingleton(tid,s1',s2',M'))) tid (tid,s1',s2',M')). 
+   econstructor. apply Union_intror. constructor. auto. eapply uniqueThreadPool in H5; eauto. 
+   inv H5. repeat constructor; auto. eqSets. 
+   {assert(tIn (tUnion T (tSingleton(tid,s1,s2,M))) x). constructor. auto. copy H5. apply H0 in H5. 
+    inversion H5; subst. auto. inv H8. exfalso. eapply uniqueTP; eauto. constructor. }
+   {assert(tIn (tUnion T' (tSingleton(tid,s1,s2,M))) x). constructor. auto. copy H5. 
+    apply H1 in H5. inversion H5; subst. auto. inv H8. exfalso. eapply uniqueTP; eauto. 
+    constructor. }
+  }
+  {subst. inv H3. repeat constructor; auto. eqSets. 
+   {assert(tIn (tUnion T (tSingleton(tid,s1,s2,M))) x). constructor. auto. copy H4. apply H0 in H4. 
+    inversion H4; subst. auto. inv H6. exfalso. eapply uniqueTP; eauto. constructor. }
+   {assert(tIn (tUnion T' (tSingleton(tid,s1,s2,M))) x). constructor. auto. copy H4. 
+    apply H1 in H4. inversion H4; subst. auto. inv H6. exfalso. eapply uniqueTP; eauto. 
+    constructor. }
+  }
+Qed. 
+
+Axiom UnionSingletonEq : forall T T' a b, 
+                 tUnion T (tSingleton a) = tUnion T' (tSingleton b) -> 
+                 tIn T' a -> T = tUnion (Subtract thread T' a) (tSingleton b).
+
+
+Theorem simSpecJoin : forall H T H' T' tid s1 s2 M' M'',
+                        spec_multistep H (tUnion T (tSingleton(tid,s1,s2,M'))) H' 
+                                       (tUnion T' (tSingleton(tid,s1,s2,M''))) ->
+                        spec_multistep H T H' T'. 
+Proof.
+  intros. dependent induction H0. 
+  {unfoldTac. apply UnionEqTID in x. invertHyp. constructor. }
+  {copy x. unfoldSetEq x. copy H. apply specStepSingleton in H4. invertHyp. 
+   assert(tIn (tUnion T0 (tSingleton x)) x). apply Union_intror. constructor.
+   apply H2 in H4. inv H4. 
+   {copy H5. apply pullOut in H5. rewrite H5. econstructor. eapply specStepChangeUnused. 
+    eauto. eapply IHspec_multistep. Focus 2. auto. apply UnionSingletonEq in H1. rewrite H1. 
+    unfoldTac. rewrite UnionSwap. auto. auto. }
+   {inv H5. inv H. 
+    {unfoldTac; invertHyp. inv H4. eapply IHspec_multistep; eauto. apply UnionEqTID in H1. 
+     invertHyp. auto. }
+     {unfoldTac; invertHyp. inv H7. eapply monotonicActions in H0. Focus 2. 
+      apply Union_intror. constructor. Focus 2. apply Union_intror. constructor.
+      destruct s1; simpl in *; omega. }
+     {unfoldTac; invertHyp. inv H4. eapply monotonicActions in H0. Focus 2. 
+      apply Union_intror. constructor. Focus 2. apply Union_intror. constructor.
+      destruct s1; simpl in *; omega. }
+     {unfoldTac; invertHyp. inv H4. eapply monotonicActions in H0. Focus 2. 
+      apply Union_intror. constructor. Focus 2. apply Union_intror. constructor.
+      destruct s1; simpl in *; omega. }
+     {unfoldTac; invertHyp. inv H4. eapply monotonicActions in H0. Focus 2. 
+      apply Union_intror. constructor. Focus 2. apply Union_intror. constructor.
+      destruct s1; simpl in *; omega. }
+     {unfoldTac; invertHyp. inv H7. eapply monotonicActions in H0. Focus 2. 
+      apply Union_intror. constructor. Focus 2. apply Union_intror. constructor.
+      destruct s1; simpl in *; omega. }
+    }
+  }
+Qed. 
+
+Inductive eraseTrm : list action -> trm -> trm -> Prop :=
+|eraseTrmNil : forall M, eraseTrm nil M M
+|eraseTrmRead : forall x t E d s M, eraseTrm (s++[rAct x t E d]) M t
+|eraseTrmWrite : forall x t E M d N s, eraseTrm (s++[wAct x t E M d]) N t
+|eraseTrmNew : forall x t E d s M, eraseTrm (s++[nAct t E d x]) M t
+|eraseTrmFork : forall t E M d N s, eraseTrm (s++[fAct t E M d]) N t
+|eraseTrmSR : forall t E M N d M' s, eraseTrm (s++[srAct t E M N d]) M' t. 
+
+Theorem unspecEraseTrm : forall tid s1 s2 M M', 
+                          eraseTrm s1 M M' ->
+                          unspecThread(tid,unlocked s1,s2,M) (tSingleton(tid,unlocked nil,s2,M')). 
+Proof.
+  intros. destructLast s1. 
+   {inv H; try invertListNeq. auto. }
+   {invertHyp. inv H; try solve[invertListNeq]; apply lastElementEq in H1;
+   subst; unspecThreadTac; auto. }
+Qed. 
+
+Theorem eEraseTrm : forall s1 M, exists M', eraseTrm s1 M M'. 
+  intros. destructLast s1. 
+  {econstructor. econstructor. }
+  {invertHyp. destruct x; econstructor; econstructor. }
+Qed. 
+
+Ltac eraseTrmTac s1 M := assert(exists M', eraseTrm s1 M M') by apply eEraseTrm; invertHyp.  
+
+Theorem EqJMeq : forall (T:Type) (x y:T), x = y -> JMeq x y.
+Proof.
+  intros. subst. auto. Qed. 
+
+
+Ltac specActEq H := 
+  eapply firstSpecActEq in H; [idtac|apply Union_intror; rewrite app_nil_l; constructor|
+                               apply Union_intror; constructor]. 
+
+Theorem wrapDistributeApp : forall s a N E e p, 
+                              wrapActs(s++[a]) N E e p = wrapActs(s) N E e p++ wrapActs[a] N E e p.
+Proof.
+  induction s; intros. 
+  {simpl. destruct a; auto. }
+  {simpl. destruct a; auto; destruct a0; auto; rewrite IHs; auto. }
+Qed. 
+
+Theorem wrapEraseTrm : forall s M M' N N' E p,
+                         eraseTrm s M M' -> 
+                         eraseTrm (wrapActs s N E N' p) 
+                                  (fill E (specJoin (ret N) M)) (fill E (specJoin (ret N) M')). 
+Proof.
+  intros. inv H; try solve[rewrite wrapDistributeApp; constructor]. 
+  {simpl. constructor. }
+Qed. 
+
+
+Theorem eraseTrmApp : forall x a M M', 
+                        eraseTrm (x ++ [a]) M M' -> actionTerm a M'. 
+Proof.
+  intros. inv H; try solve[apply lastElementEq in H1; subst; constructor].
+  invertListNeq. 
+Qed. 
+
+Theorem specFastForward : forall H T H' T' tid x0 x s2' N N0 M M' M'',
+    eraseTrm (x0++[x]) N M' ->                                                
+    spec_multistep H (tUnion T (tSingleton(tid,specStack nil N0, s2', M)))
+                   H' (tUnion T' (tSingleton(tid,specStack(x0++[x]) N0, s2', M''))) ->
+    exists H'' T'',
+      spec_multistep H (tUnion T (tSingleton(tid,specStack nil N0, s2', M))) 
+                     H'' (tUnion T'' (tSingleton(tid,specStack nil N0, s2', M'))) /\
+      spec_multistep H'' (tUnion T'' (tSingleton(tid, specStack nil N0, s2', M')))
+                     H' (tUnion T' (tSingleton(tid,specStack(x0++[x]) N0, s2',M''))). 
+Proof.
+  intros. dependent induction H1. 
+  {apply UnionEqTID in x. invertHyp. inv H. invertListNeq. }
+  {copy x. unfoldSetEq H2. copy H. apply specStepSingleton in H2. invertHyp. 
+   assert(tIn (tUnion T0 (tSingleton x2)) x2). apply Union_intror. constructor. apply H3 in H2. 
+   inv H2. 
+   {eapply IHspec_multistep in H0. Focus 3. auto. Focus 2. apply UnionSingletonEq in x; auto.  
+    rewrite x. unfoldTac. rewrite UnionSwap. auto. invertHyp. exists x3. exists x4. split; auto.
+    apply pullOut in H5. unfoldTac. rewrite H5. rewrite UnionSwap. econstructor. 
+    eapply specStepChangeUnused. eauto. unfoldTac. rewrite <- UnionSwap. eauto. }
+   {inv H5. apply UnionEqTID in x. invertHyp. clear H2 H5 H7. inversion H; subst. 
+    {unfoldTac; invertHyp. inv H2. eapply IHspec_multistep in H0. Focus 3. 
+     auto. Focus 2. auto. invertHyp. exists x. exists x2. split; eauto. econstructor. 
+     eapply SBasicStep; eauto. assumption. }
+    {unfoldTac; invertHyp. inv H7. copy H1. specActEq H1. subst. 
+     apply eraseTrmApp in H0. inv H0.  exists h'. exists T. split. constructor. 
+     econstructor. eapply SFork. eauto. }
+    {unfoldTac; invertHyp. inv H2. copy H1. specActEq H1. subst. exists h. exists T. 
+     apply eraseTrmApp in H0. inv H0. split. constructor. econstructor. 
+     eauto. eauto. }
+    {unfoldTac; invertHyp. inv H2. copy H1. specActEq H1. subst. exists h. exists T. 
+     apply eraseTrmApp in H0. inv H0. split. constructor. econstructor. 
+     eauto. eauto. }
+    {unfoldTac; invertHyp. inv H2. copy H1. specActEq H1. subst. exists h. exists T. 
+     apply eraseTrmApp in H0. inv H0. split. constructor. econstructor. 
+     eauto. eauto. }
+    {unfoldTac; invertHyp. inv H7. copy H1. specActEq H1. subst. apply eraseTrmApp in H0. 
+     inv H0. exists h'. exists T. split. constructor. econstructor. eauto. eauto. }
+   }
+  }
+Qed. 
+
+Ltac monoActs H :=
+  eapply monotonicActions in H;[idtac|apply Union_intror; constructor|apply Union_intror;constructor].
+
+Theorem simTSteps : forall H T H' T' tid s1 s2 s1' s2' N M M' tid',
+                      spec_multistep H (tUnion T (tSingleton(tid,s1,s2,M)))
+                                     H' (tUnion T' (tSingleton(tid,s1,s2,M'))) ->
+                      spec_multistep H (tUnion T (tSingleton(tid',s1',s2',N)))
+                                     H' (tUnion T' (tSingleton(tid',s1',s2',N))). 
+Proof.
+  intros. dependent induction H0. 
+  {apply UnionEqTID in x. invertHyp. constructor. }
+  {copy x. unfoldSetEq x. copy H. apply specStepSingleton in H4. invertHyp. 
+   assert(tIn (tUnion T0 (tSingleton x)) x). apply Union_intror. constructor. 
+   apply H2 in H4. inv H4. 
+   {copy H5. apply pullOut in H5. rewrite H5. unfoldTac. rewrite UnionSwap. econstructor. 
+    eapply specStepChangeUnused. eauto. unfoldTac. rewrite <- UnionSwap.
+    eapply IHspec_multistep; eauto. apply UnionSingletonEq in H1. rewrite H1.
+    rewrite UnionSwap. eauto. auto. }
+   {inv H5. inv H; unfoldTac; invertHyp; invThreadEq.   
+    {eapply IHspec_multistep; eauto. apply UnionEqTID in H1. invertHyp. eauto. }
+    {monoActs H0. destruct s1; simpl in *; omega. }
+    {monoActs H0. destruct s1; simpl in *; omega. }
+    {monoActs H0. destruct s1; simpl in *; omega. }
+    {monoActs H0. destruct s1; simpl in *; omega. }
+    {monoActs H0. destruct s1; simpl in *; omega. }
+   }
+  }
+Qed. 
+
+
+Fixpoint joinCtxts E1 E2 :=
+  match E1 with
+      | bindCtxt E M => bindCtxt (joinCtxts E E2) M
+      | handleCtxt E M => handleCtxt (joinCtxts E E2) M
+      | appCtxt E M => appCtxt (joinCtxts E E2) M
+      | appValCtxt E M => appValCtxt (joinCtxts E E2) M
+      | pairCtxt E M => pairCtxt (joinCtxts E E2) M
+      | pairValCtxt E M => pairValCtxt (joinCtxts E E2) M
+      | fstCtxt E => fstCtxt (joinCtxts E E2)
+      | sndCtxt E => sndCtxt (joinCtxts E E2)
+      | specRunCtxt E M => specRunCtxt (joinCtxts E E2) M
+      | specJoinCtxt E M => specJoinCtxt (joinCtxts E E2) M
+      | holeCtxt => E2
+  end. 
+
+Theorem notValFill : forall E e, ~ val e -> ~val (fill E e). 
+Proof.
+  induction E; intros; simpl; try solve[introsInv].
+  {intros c. inv c. apply IHE in H. contradiction. }
+  {intros c. inv c. apply IHE in H. contradiction. }
+  {auto. }
+Qed. 
+
+Theorem decomposeNotVal : forall t E e, decompose t E e -> E <> holeCtxt -> ~val t. 
+Proof.
+  intros. induction H; try solve[introsInv].
+  {intros c. inv c. contradiction. }
+  {introsInv. contradiction. }
+Qed. 
+
+Theorem decomposeFurther : forall E E' e e' e'',
+                                  ctxtWF e E -> decompose e' E' e'' -> ~ val e' ->
+                                  decompose (fill E e') (joinCtxts E E') e''.
+Proof.
+  induction E; intros. 
+  {simpl. constructor. inv H. eapply notValFill. auto. inv H. eapply IHE; eauto. }
+  {simpl. inv H. constructor. auto. apply notValFill; auto. eauto. }
+  {inv H. simpl. constructor; eauto. apply notValFill; eauto. }
+  {inv H. simpl. constructor; eauto. apply notValFill; eauto. }
+  {inv H. simpl. constructor; eauto. apply notValFill; eauto. }
+  {inv H. simpl. constructor; eauto. apply notValFill; eauto. }
+  {inv H. simpl. constructor; eauto. apply notValFill; eauto. }
+  {inv H. simpl. constructor; eauto. apply notValFill; eauto. }
+  {inv H. simpl. constructor; eauto. apply notValFill; eauto. }
+  {inv H. simpl. constructor; eauto. apply notValFill; eauto. }
+  {simpl. auto. }
+Qed. 
+
+
+Theorem joinFill : forall E1 E2 e, fill (joinCtxts E1 E2) e = fill E1 (fill E2 e). 
+Proof.
+  induction E1; intros; try solve[simpl; rewrite IHE1; eauto]. 
+  simpl. auto. 
+Qed. 
+
+Theorem decomposeJoin : forall e e' e'' E E', 
+                          ctxtWF e E -> decompose e' E' e'' -> ~val e'' ->
+                          decompose (fill E e') (joinCtxts E E') e''. 
+Proof.
+  intros. induction H; try solve[
+  simpl; constructor; auto; apply decomposeEq in H0; subst;
+  repeat apply notValFill; auto].
+  {simpl. auto. }
+Qed. 
+
+Theorem fillDecompose : forall E t E' e' x,
+                          decompose t E' e' -> ctxtWF x E -> ~val e' ->
+                          fill E t = fill (joinCtxts E E') e' /\
+                          decompose (fill (joinCtxts E E') e') (joinCtxts E E') e'. 
+Proof.
+  induction E; intros. 
+  {simpl. inv H0. eapply IHE in H; eauto. invertHyp. split. rewrite H0. auto. 
+   constructor. apply notValFill. auto. auto. }
+  {simpl. inv H0. eapply IHE in H; eauto. invertHyp. split. rewrite H0. auto. 
+   constructor; auto. apply notValFill. auto. }
+  {simpl. inv H0. eapply IHE in H; eauto. invertHyp. split. rewrite H0. auto. 
+   constructor; auto. apply notValFill. auto. }
+  {simpl. inv H0. eapply IHE in H; eauto. invertHyp. split. rewrite H0. auto. 
+   constructor; auto. apply notValFill. auto. }
+  {simpl. inv H0. eapply IHE in H; eauto. invertHyp. split. rewrite H0. auto. 
+   constructor; auto. apply notValFill. auto. }
+  {simpl. inv H0. eapply IHE in H; eauto. invertHyp. split. rewrite H0. auto. 
+   constructor; auto. apply notValFill. auto. }
+  {simpl. inv H0. eapply IHE in H; eauto. invertHyp. split. rewrite H0. auto. 
+   constructor; auto. apply notValFill. auto. }
+  {simpl. inv H0. eapply IHE in H; eauto. invertHyp. split. rewrite H0. auto. 
+   constructor; auto. apply notValFill. auto. }
+  {simpl. inv H0. eapply IHE in H; eauto. invertHyp. split. rewrite H0. auto. 
+   constructor; auto. apply notValFill. auto. }
+  {simpl. inv H0. eapply IHE in H; eauto. invertHyp. split. rewrite H0. auto. 
+   constructor; auto. apply notValFill. auto. }
+  {simpl. copy H. apply decomposeEq in H. subst. split; auto. }
+Qed. 
+
+Theorem basicStepNotVal : forall M M', 
+                            basic_step M M' -> ~val M. 
+Proof.
+  intros. inv H;
+          try solve[apply decomposeEq in H0; subst; apply notValFill; introsInv].
+Qed.  
+ 
+Theorem subtractSingle : forall X T x1, 
+              (Subtract X (Union X (Subtract X T x1) (Singleton X x1)) x1) =
+              Subtract X T x1. 
+Proof.
+  intros. eqSets. 
+  {inv H. inv H0. auto. inv H. exfalso. apply H1. constructor. }
+  {inv H. constructor. constructor. constructor. auto. auto. auto. }
+Qed. 
+Theorem nonEmptyStack : forall s1 s1' s2 x M M' tid N H H' T T' z,
+        eraseTrm (s1'++[x]) z M' ->
+        spec_multistep H (tUnion T (tSingleton(tid,specStack nil N,s2, M')))
+                       H' (tUnion T' (tSingleton(tid,specStack s1 N,s2,M))) ->
+        M <> M' -> s1 <> nil. 
+Proof. 
+  intros. dependent induction H1.  
+  {Admitted. 
+
+Ltac replaceTac :=
+     match goal with
+         | |- basic_step _ (fill ?E (specJoin ?x (fill ?E' ?y))) =>
+           replace (specJoin x (fill E' y)) with (fill (specJoinCtxt E' x) y); auto
+     end. 
+
+Theorem simBasicStep' : forall M M' N1 E e,
+                          basic_step M M' -> ctxtWF e E -> ~val M -> 
+                          basic_step (fill E (specJoin (ret N1) M))
+                                     (fill E (specJoin (ret N1) M')).
+Proof.
+  intros. inv H. 
+  {eapply fillDecompose in H0. invertHyp. rewrite H. Focus 2. constructor; 
+   auto. eauto. replaceTac. rewrite <- joinFill. econstructor. eauto. introsInv. }
+  {eapply fillDecompose in H0. invertHyp. rewrite H. Focus 2. constructor; eauto. 
+   replaceTac. rewrite <- joinFill. econstructor. eauto. introsInv. }
+  {eapply fillDecompose in H0. invertHyp. rewrite H. Focus 2. constructor; eauto. 
+   replaceTac. rewrite <- joinFill. eapply basicProjR. eauto. introsInv. }
+  {eapply fillDecompose in H0. invertHyp. rewrite H. Focus 2. constructor; eauto. 
+   replaceTac. rewrite <- joinFill. eapply basicBind. eauto. introsInv. }
+  {eapply fillDecompose in H0. invertHyp. rewrite H. Focus 2. constructor; eauto. 
+   replaceTac. rewrite <- joinFill. eapply basicBindRaise. eauto. introsInv. }
+  {eapply fillDecompose in H0. invertHyp. rewrite H. Focus 2. constructor; eauto. 
+   replaceTac. rewrite <- joinFill. eapply basicHandle. eauto. introsInv. }
+  {eapply fillDecompose in H0. invertHyp. rewrite H. Focus 2. constructor; eauto. 
+   replaceTac. rewrite <- joinFill. eapply basicHandleRet. eauto. introsInv. }
+Qed. 
+
+Theorem basicStepNeq : forall s1 x M M' M'' x0,
+                         eraseTrm (s1++[x]) M x0 ->
+                         basic_step M' M'' -> x0 <> M'. 
+Proof.
+  intros. inv H0; inv H; try solve[invertListNeq];
+  apply lastElementEq in H2; subst; intros c; subst; eapply uniqueCtxtDecomp in H1; eauto; invertHyp; solveByInv. 
+Qed.   
+
+Theorem simSpecJoin' : forall H T H' T' H'' T'' tid tid' s2 s2' M M' y s1 s1' N0 N1 E e p x z,  
+        eraseTrm (s1'++[y]) z x ->                 
+        spec_multistep H'' (tUnion T'' (tSingleton(tid,specStack nil N0, s2, x))) 
+                       H (tUnion T (tSingleton(tid,specStack s1 N0,s2,M))) -> 
+        spec_multistep H (tUnion T (tSingleton(tid,specStack s1 N0, s2, M)))
+                       H' (tUnion T' (tSingleton(tid,specStack(s1'++[y]) N0, s2, M'))) -> ~val e ->
+        spec_multistep H (tUnion T (tSingleton(tid',unlocked (wrapActs s1 N1 E e p),s2',fill E (specJoin(ret N1)M))))
+           H' (tUnion T' (tSingleton(tid',unlocked(wrapActs(s1'++[y]) N1 E e p),s2',fill E (specJoin(ret N1)M')))).
+Proof.
+  intros. dependent induction H2. 
+  {apply UnionEqTID in x. invertHyp. inv H. constructor. }
+  {copy x. unfoldSetEq H4. copy H. apply specStepSingleton in H4. invertHyp. 
+   assert(tIn (tUnion T0 (tSingleton x1)) x1). apply Union_intror. constructor. 
+   apply H5 in H4. inv H4. 
+   {copy H7. apply pullOut in H7. rewrite H7. unfoldTac. rewrite UnionSwap. 
+    econstructor. eapply specStepChangeUnused. eauto. unfoldTac. 
+    rewrite <- UnionSwap. eapply IHspec_multistep; eauto. eapply spec_multi_trans. 
+    eassumption. rewrite H7. rewrite UnionSwap. econstructor. 
+    eapply specStepChangeUnused. eauto. rewrite subtractSingle. rewrite UnionSwap. 
+    constructor. apply UnionSingletonEq in x. rewrite x. unfoldTac. 
+    rewrite UnionSwap. auto. auto. }
+   {inv H7. apply UnionEqTID in x. invertHyp. 
+    inv H; unfoldTac; invertHyp; invThreadEq.  
+    {copy H10. eapply simBasicStep' in H; eauto. Focus 2. copy H.
+     apply basicStepNotVal in H. auto. econstructor. eapply SBasicStep; eauto.
+     eapply nonEmptyStack in H1. destruct s1. exfalso; apply H1. auto. 
+     destruct a; simpl; constructor. eauto. eapply basicStepNeq in H10; eauto. 
+     eapply IHspec_multistep; eauto. eapply spec_multi_trans. eassumption. 
+     econstructor. eapply SBasicStep. eauto. eauto. constructor. }
+    {econstructor. Admitted. 
+
+
+ 
+
+
+
+
+
